Surface/Global.lean
@@ -84,11 +84,11 @@ def Entry.kind : Entry -> Option Core.Kind
 def lookup (x : String) : GlobalEnv -> Option (Entry)
 | [] => none
 | .cons (.data (n := n) y K ctors) tl =>
-  let ctors' : Fun.Vec (Option (Entry)) n := λ i =>
-    let (z, A) := ctors.to i
-    if x == z then return .ctor z i A else none
+  let ctors' := Vec.map
+    (λ ((z, A), i) => if x == z then some (Entry.ctor z i A) else none)
+    (Vec.zipIdx ctors)
   if x == y then return .data y K ctors
-  else ctors'.to.foldl (init := lookup x tl) Option.or
+  else ctors'.foldr (init := lookup x tl) Option.or
 | .cons (.defn y a b) tl =>
   if x == y then return .defn y a b else lookup x tl
 | .cons (.classDecl (kc := kc) y Ks /-scs fds-/ ms) tl =>
@@ -145,14 +145,15 @@ theorem lookup_name_agrees : lookup x G = some e -> e.name = x := by
   all_goals try solve | subst h; simp [Entry.name]
   case _ n y K ctors tl ctors' h2 ih =>
     generalize zdef : lookup x tl = z at *
-    replace h := Vec.fold_or h
+    replace h := Vec.foldr_or h
     cases h
-    case _ h => apply ih h
     case _ h =>
       rcases h with ⟨j, h⟩
-      subst ctors'; simp [Vec.get_to] at h
+      subst ctors'; simp at h
       rcases h with ⟨h1, h3⟩; subst h1
       subst e; simp[Entry.name]
+    case _ h =>
+      apply ih h.2
   case _ ms_mb ms _ =>
     simp [ms, ms_mb] at h; rcases h with ⟨a, b, h, h1⟩
     simp [<-h1, Entry.name]; subst e; simp [List.find?_eq_some_iff_getElem] at h; symm; apply h.1
